Checkpoint state proof

src/program_proof/simplepb/state_proof.v
@@ -1,6 +1,7 @@
 From Perennial.program_proof Require Import grove_prelude.
 From Goose.github_com.mit_pdos.gokv.simplepb Require Import state.
 From Perennial.program_proof.simplepb Require Import pb_definitions.
+From Perennial.program_proof Require Import marshal_stateless_proof.
 From iris.base_logic Require Import ghost_map.
 
 Section state_proof.
@@ -9,29 +10,103 @@ Context `{!heapGS Σ, !pbG Σ}.
 
 Implicit Type σ : list (list u8).
 
-Definition own_kvs (γkv:gname) σ : iProp Σ.
-Admitted.
+Context `{!ghost_mapG Σ u64 (list u8)}.
+Definition own_kvs (γkv:gname) σ : iProp Σ :=
+  (* TODO: m has to agree with σ *)
+  ∃ m,
+  ghost_map_auth γkv 1 m.
 
 Definition sys_inv γ γkv : iProp Σ :=
   inv pbN ( ∃ σ, own_ghost γ σ ∗ own_kvs γkv σ).
 
-Context `{!ghost_mapG Σ u64 (list u8)}.
 Definition kv_ptsto γkv (k:u64) (v:list u8): iProp Σ :=
   k ↪[γkv] v.
 
-Lemma wp_Clerk__FetchAndAppend ck γkv key val_sl value Φ:
+Definition is_Clerk ck : iProp Σ :=
+  ∃ (cl:loc),
+    "#Hcl" ∷ readonly (ck ↦[state.Clerk :: "cl"] #cl).
+
+(* FIXME: this belongs in pb *)
+Context `{!urpc_proof.urpcregG Σ}.
+Context `{!stagedG Σ}.
+Lemma wp_Clerk__PrimaryApply γ ck op_sl op (Φ:val → iProp Σ) :
+is_slice op_sl byteT 1 op -∗
+(|={⊤,∅}=> ∃ σ, own_ghost γ σ ∗
+  (own_ghost γ (σ ++ [op]) ={∅,⊤}=∗
+(∀ reply_sl, is_slice reply_sl byteT 1 (replyFn σ) -∗
+    Φ (slice_val reply_sl))))
+    -∗
+WP Clerk__PrimaryApply #ck (slice_val op_sl) {{ Φ }}.
+Proof.
+Admitted.
+
+Lemma wp_Clerk__FetchAndAppend ck γ γkv key val_sl value Φ:
+  sys_inv γ γkv -∗
+  is_Clerk ck -∗
   is_slice val_sl byteT 1 value -∗
-  (|={⊤,∅}=> ∃ old_value, kv_ptsto γkv key old_value ∗
-    (kv_ptsto γkv key (old_value ++ value) ={∅,⊤}=∗
+  (|={⊤∖↑pbN,∅}=> ∃ old_value, kv_ptsto γkv key old_value ∗
+    (kv_ptsto γkv key (old_value ++ value) ={∅,⊤∖↑pbN}=∗
   (∀ reply_sl, is_slice reply_sl byteT 1 old_value -∗
       Φ (slice_val reply_sl))))
   -∗
-  WP state.Clerk__FetchAndAppend #ck #key (slice_val val_sl) @ ⊤ {{ Φ }}.
+  WP state.Clerk__FetchAndAppend #ck #key (slice_val val_sl) {{ Φ }}.
 Proof.
-  iIntros "Hval_sl Hupd".
+  iIntros "#Hinv #Hck Hval_sl Hupd".
   wp_call.
   wp_pures.
+  wp_apply (wp_slice_len).
+  wp_pures.
+  wp_apply (wp_NewSliceWithCap).
+  { admit. }
+  iIntros (op) "Hop_sl".
+  set op_sl:=(Slice.mk _ _ _).
+  wp_apply (wp_ref_to).
+  { done. }
+  replace (int.nat 0%Z) with (0) by word.
+  simpl.
+  iIntros (op_ptr) "Hop_ptr".
+  wp_pures.
+  wp_load.
+  wp_apply (wp_WriteInt with "Hop_sl").
+  iIntros (op_sl') "Hop_sl".
+  wp_store.
+  clear op_sl.
+  simpl.
 
+  wp_load.
+  wp_apply (wp_WriteBytes with "[$Hop_sl Hval_sl]").
+  {
+    iDestruct (is_slice_to_small with "Hval_sl") as "$".
+  }
+  iIntros (op_sl) "[Hop_sl Hval_sl]".
+  wp_store.
+  clear op_sl'.
+  wp_load.
+  iNamed "Hck".
+  wp_loadField.
+
+  wp_apply (wp_Clerk__PrimaryApply with "Hop_sl").
+  iInv "Hinv" as ">Hown" "Hclose".
+  iMod "Hupd".
+  iModIntro.
+
+  iDestruct "Hown" as (?) "[Hown Hkvs]".
+  iExists _.
+  iFrame.
+
+  iIntros "Hghost".
+  iMod (fupd_mask_subseteq).
+  { admit. } (* FIXME: the masks are wrong *)
+  (* need to update own_kvs; need to fire Hupd *)
+  iMod ("Hclose" with "[Hghost Hkvs]") as "HH".
+  {
+    iNext.
+    iExists _; iFrame "Hghost".
+    admit.
+  }
+  iModIntro.
+  iIntros (reply_sl) "Hreply_sl".
+  admit.
 Admitted.
 
 End state_proof.
